example/Deed.thy
@@ -16,13 +16,7 @@ $ solc/solc --bin-runtime
 abbreviation deed :: "char list"
 where "deed == ''6060604052361561006c5760e060020a600035046305b34410811461006e5780630b5ab3d51461007c57806313af4035146100895780632b20e397146100af5780638da5cb5b146100c6578063bbe42771146100dd578063faab9d3914610103578063fb1669ca14610129575b005b346100025761014a60015481565b346100025761006c610189565b346100025761006c60043560005433600160a060020a039081169116146101f857610002565b34610002576101a0600054600160a060020a031681565b34610002576101a0600254600160a060020a031681565b346100025761006c60043560005433600160a060020a0390811691161461025757610002565b346100025761006c60043560005433600160a060020a039081169116146102c757610002565b61006c60043560005433600160a060020a039081169116146102e957610002565b60408051918252519081900360200190f35b6040517fbb2ce2f51803bba16bc85282b47deeea9a5c6223eabea1077be696b3f265cf1390600090a16102545b60025460a060020a900460ff16156101bd57610002565b60408051600160a060020a03929092168252519081900360200190f35b604051600254600160a060020a0390811691309091163180156108fc02916000818181858888f19350505050156101f35761deadff5b610002565b6002805473ffffffffffffffffffffffffffffffffffffffff19168217905560408051600160a060020a038316815290517fa2ea9883a321a3e97b8266c2b078bfeec6d50c711ed71f874a90d500ae2eaf369181900360200190a15b50565b60025460a060020a900460ff16151561026f57610002565b6002805474ff00000000000000000000000000000000000000001916905560405161dead906103e830600160a060020a031631848203020480156108fc02916000818181858888f19350505050151561015c57610002565b6000805473ffffffffffffffffffffffffffffffffffffffff19168217905550565b60025460a060020a900460ff16151561030157610002565b8030600160a060020a031631101561031857610002565b600254604051600160a060020a039182169130163183900380156108fc02916000818181858888f1935050505015156102545761000256''"
 *)
-
-abbreviation deed :: "char list"
-where "deed == ''6060604052361561006c5760e060020a600035046305b34410811461006e5780630b5ab3d51461007c57806313af4035146100895780632b20e397146100af5780638da5cb5b146100c6578063bbe42771146100dd5780''"
-
-
-definition deed_bytes :: "byte list"
-where deed_b [simplified, simp]: "deed_bytes == bytes_of_hex_content deed"
+(* it seems like the storage index 0 contains the registrar *)
 
 value [simp] "deed_bytes"
 
@@ -616,39 +610,26 @@ lemma deed_keeps_invariant :
 "no_assertion_failure deed_inv"
 apply(simp only: no_assertion_failure_def)
 apply(rule allI)
+apply(rule allI)
 apply(rule impI)
 apply(rule impI)
 apply(rule allI)
 apply(rule impI)
 apply(drule star_case; auto)
-       apply(case_tac steps; auto)
-       apply(split if_splits; auto)
-        apply(drule star_case; auto)
-       apply(split strict_if_split; auto)
-        apply(drule star_case; auto)
-       apply(split strict_if_split; auto)
-        apply(drule star_case; auto)
-       apply(drule star_case; auto)
-      apply(case_tac steps; auto)
-      apply(split strict_if_split; auto)
-       apply(split strict_if_split; auto)
-        apply(drule star_case; auto)
-       apply(split strict_if_split; auto)
-        apply(drule star_case; auto)
-       apply(drule star_case; auto)
-      apply(drule star_case; auto)
      apply(case_tac steps; auto)
+     apply(split if_splits; auto)
+      apply(split if_splits; auto)
      apply(split strict_if_split; auto)
-     apply(split strict_if_split; auto)
-     apply(split strict_if_split; auto)
-    apply(case_tac steps; auto)
-    apply(split strict_if_split; auto)
-    apply(split strict_if_split; auto)
-   apply(split strict_if_split; auto)
-   apply(case_tac steps; auto)
-  apply(case_tac steps; auto)
- apply(case_tac steps; auto)
-apply(case_tac steps; auto)
+      apply(split if_splits; auto)
+     
 done
+
+lemma deed_only_registrar_can_spend :
+"pre_post_conditions deed_inv
+ (\<lambda> init_state init_call. account_storage init_state 0 \<noteq> ucast (callenv_caller init_call))
+ (\<lambda> init_state _ (post_state, _). account_balance init_state \<le> account_balance post_state)
+"
+
+
 
 end
